Start adding support for a call stack
Get the test_storage_array_assign test working, and move all the tests
to be tests of external calls (not just function body execution)

vyperTestScript.sml
@@ -7,31 +7,32 @@ val () = new_theory "vyperTest";
 Overload uint256 = “BaseT (UintT (n2w (256 DIV 8)))”
 
 Definition test_if_control_flow_ast_def:
-  test_if_control_flow_ast =
-  FunctionDef "foo" [External] [] uint256
-  [
-    AnnAssign "a" uint256 (Literal (IntL 1));
-    If (Compare (Name "a") Eq (Literal (IntL 1)))
+  test_if_control_flow_ast = [
+    FunctionDef "foo" External [] uint256
     [
-      Assign (BaseTarget (NameTarget "a")) (Literal (IntL 2))
+      AnnAssign "a" uint256 (Literal (IntL 1));
+      If (Compare (Name "a") Eq (Literal (IntL 1)))
+      [
+        Assign (BaseTarget (NameTarget "a")) (Literal (IntL 2))
+      ]
+      [
+        Assign (BaseTarget (NameTarget "a")) (Literal (IntL 3))
+      ];
+      Return (SOME (BinOp (Name "a") Add (Literal (IntL 42))))
     ]
-    [
-      Assign (BaseTarget (NameTarget "a")) (Literal (IntL 3))
-    ];
-    Return (SOME (BinOp (Name "a") Add (Literal (IntL 42))))
   ]
 End
 
-Theorem evaluate_test_if_control_flow_body:
-  execute_stmts 10
-    (function_body test_if_control_flow_ast)
-    initial_function_context = result_ctx
-  ==>
-  result_ctx.raised = SOME (ReturnException (IntV 44))
+Theorem test_if_control_flow:
+  external_call 10 "foo" [] test_if_control_flow_ast
+  = SOME (ReturnException (IntV 44))
 Proof
-  rw[function_body_def, test_if_control_flow_ast_def]
-  \\ simp[execute_stmts_def, new_variable_def,
-          initial_function_context_def, assign_subscripts_def,
+  rw[external_call_def,
+     test_if_control_flow_ast_def,
+     lookup_external_function_def, bind_arguments_def,
+     initial_execution_context_def, initial_globals_def,
+     initial_function_context_def ]
+  \\ simp[execute_stmts_def, new_variable_def, assign_subscripts_def,
           evaluate_exps_def, assign_target_def, set_variable_def,
           evaluate_target_def, evaluate_base_target_def,
           evaluate_cmp_def, evaluate_literal_def,
@@ -41,28 +42,29 @@ Proof
 QED
 
 Definition test_for_control_flow_ast_def:
-  test_for_control_flow_ast =
-  FunctionDef "foo" [External] [] uint256
-  [
-     AnnAssign "a" (DynArrayT uint256 10)
-       (ArrayLit [Literal (IntL 1); Literal (IntL 2); Literal (IntL 3)]);
-     AnnAssign "counter" uint256 (Literal (IntL 0));
-     For "i" uint256 (Name "a")
-     [ AugAssign "counter" Add (Name "i") ];
-     Return (SOME (Name "counter"))
+  test_for_control_flow_ast = [
+    FunctionDef "foo" External [] uint256
+    [
+       AnnAssign "a" (DynArrayT uint256 10)
+         (ArrayLit [Literal (IntL 1); Literal (IntL 2); Literal (IntL 3)]);
+       AnnAssign "counter" uint256 (Literal (IntL 0));
+       For "i" uint256 (Name "a")
+       [ AugAssign "counter" Add (Name "i") ];
+       Return (SOME (Name "counter"))
+    ]
   ]
 End
 
-Theorem evaluate_test_for_control_flow_body:
-  execute_stmts 10
-    (function_body test_for_control_flow_ast)
-    initial_function_context = result_ctx
-  ==>
-  result_ctx.raised = SOME (ReturnException (IntV 6))
+Theorem test_for_control_flow:
+  external_call 10 "foo" [] test_for_control_flow_ast
+  = SOME (ReturnException (IntV 6))
 Proof
-  rw[function_body_def, test_for_control_flow_ast_def]
-  \\ simp[execute_stmts_def,
-       initial_function_context_def, new_variable_def,
+  rw[external_call_def,
+     test_for_control_flow_ast_def,
+     lookup_external_function_def, bind_arguments_def,
+     initial_execution_context_def, initial_globals_def,
+     initial_function_context_def ]
+  \\ simp[execute_stmts_def, new_variable_def,
        set_variable_def, evaluate_base_target_def, evaluate_target_def,
        evaluate_exps_def, assign_target_def,
        evaluate_cmp_def, evaluate_literal_def,
@@ -72,29 +74,30 @@ Proof
 QED
 
 Definition test_array_assign_ast_def:
-  test_array_assign_ast =
-  FunctionDef "foo" [External] [] uint256
-  [
-    AnnAssign "bar" (DynArrayT uint256 10)
-      (ArrayLit [Literal (IntL 1); Literal (IntL 2)]);
-    Assign (BaseTarget (SubscriptTarget (NameTarget "bar") (Literal (IntL 0))))
-      (Literal (IntL 3));
-    Return (SOME (BinOp (BinOp (Subscript (Name "bar") (Literal (IntL 0))) Add
-                               (Subscript (Name "bar") (Literal (IntL 1)))) Add
-                        (Literal (IntL 42))))
+  test_array_assign_ast = [
+    FunctionDef "foo" External [] uint256
+    [
+      AnnAssign "bar" (DynArrayT uint256 10)
+        (ArrayLit [Literal (IntL 1); Literal (IntL 2)]);
+      Assign (BaseTarget (SubscriptTarget (NameTarget "bar") (Literal (IntL 0))))
+        (Literal (IntL 3));
+      Return (SOME (BinOp (BinOp (Subscript (Name "bar") (Literal (IntL 0))) Add
+                                 (Subscript (Name "bar") (Literal (IntL 1)))) Add
+                          (Literal (IntL 42))))
+    ]
   ]
 End
 
-Theorem evaluate_test_array_assign_body:
-  execute_stmts 10
-    (function_body test_array_assign_ast)
-    initial_function_context = result_ctx
-  ==>
-  result_ctx.raised = SOME (ReturnException (IntV 47))
+Theorem test_array_assign:
+  external_call 10 "foo" [] test_array_assign_ast
+  = SOME (ReturnException (IntV 47))
 Proof
-  rw[function_body_def, test_array_assign_ast_def]
-  \\ simp[execute_stmts_def,
-       initial_function_context_def, new_variable_def,
+  rw[external_call_def,
+     test_array_assign_ast_def,
+     lookup_external_function_def, bind_arguments_def,
+     initial_execution_context_def, initial_globals_def,
+     initial_function_context_def ]
+  \\ simp[execute_stmts_def, new_variable_def,
        set_variable_def, evaluate_base_target_def, evaluate_target_def,
        evaluate_exps_def, assign_target_def, add_subscript_def,
        assign_subscripts_def, extract_elements_def, replace_elements_def,
@@ -104,13 +107,10 @@ Proof
        raise_def, FLOOKUP_UPDATE]
 QED
 
-(* TODO: evaluate a list of toplevels to a contract context (globals + functions) *)
-(* TODO: make the tests evaluate an external call in a given context *)
-
 Definition test_storage_array_assign_ast_def:
   test_storage_array_assign_ast = [
     VariableDecl "a" (DynArrayT uint256 10) Private Storage;
-    FunctionDef "foo" [External] [] uint256 [
+    FunctionDef "foo" External [] uint256 [
       Assign (BaseTarget (GlobalNameTarget "a"))
         (ArrayLit [Literal (IntL 1); Literal (IntL 2)]);
       Assign (BaseTarget
@@ -124,5 +124,24 @@ Definition test_storage_array_assign_ast_def:
     ]
   ]
 End
+
+Theorem test_storage_array_assign:
+  external_call 10 "foo" [] test_storage_array_assign_ast
+  = SOME (ReturnException (IntV 5))
+Proof
+  rw[external_call_def,
+     test_storage_array_assign_ast_def,
+     lookup_external_function_def, bind_arguments_def,
+     initial_execution_context_def, initial_globals_def,
+     initial_function_context_def ]
+  \\ simp[execute_stmts_def, new_variable_def,
+       set_variable_def, evaluate_base_target_def, evaluate_target_def,
+       evaluate_exps_def, assign_target_def, add_subscript_def,
+       assign_subscripts_def, extract_elements_def, replace_elements_def,
+       evaluate_cmp_def, evaluate_literal_def, integer_index_def,
+       evaluate_binop_def, push_scope_def, lookup_scopes_def,
+       find_containing_scope_def, pop_scope_def,
+       raise_def, FLOOKUP_UPDATE]
+QED
 
 val () = export_theory();
